Impl/StateSectorModel.i.dfy
@@ -6,6 +6,8 @@ module StateSectorModel {
   import BT = PivotBetreeSpec`Internal
   import IndirectionTableModel
   import SectorType
+  import BC = BlockCache
+  import JC = JournalCache
 
   type Node = BT.G.Node  
   type IndirectionTable = IndirectionTableModel.IndirectionTable
@@ -14,4 +16,27 @@ module StateSectorModel {
     | SectorNode(node: Node)
     | SectorIndirectionTable(indirectionTable: IndirectionTable)
     | SectorSuperblock(superblock: SectorType.Superblock)
+
+  predicate WFNode(node: Node)
+  {
+    BT.WFNode(node)
+  }
+  
+  predicate WFSector(sector: Sector)
+  {
+    match sector {
+      case SectorNode(node) => WFNode(node)
+      case SectorIndirectionTable(indirectionTable) => (
+        && IndirectionTableModel.Inv(indirectionTable)
+        && BC.WFCompleteIndirectionTable(IIndirectionTable(indirectionTable))
+      )
+      case SectorSuperblock(superblock) =>
+        JC.WFSuperblock(superblock)
+    }
+  }
+
+  function IIndirectionTable(table: IndirectionTable) : (result: SectorType.IndirectionTable)
+  {
+    IndirectionTableModel.I(table)
+  }
 }
